src/proofs/no_slashable_attestations/supporting_lemmas/fnc_invs_1_26.dfy
@@ -783,21 +783,21 @@ module Fnc_Invs_1_26
         }
     }
 
-    lemma lemma_inv8_f_start_next_duty(process: DVCState, attestation_duty: AttestationDuty, process': DVCState)
+    lemma lemma_inv_none_latest_served_duty_implies_none_current_att_duty_f_start_next_duty(process: DVCState, attestation_duty: AttestationDuty, process': DVCState)
     requires f_start_next_duty.requires(process, attestation_duty)
     requires process' == f_start_next_duty(process, attestation_duty).state        
-    requires inv8_body(process)
-    ensures inv8_body(process')
+    requires inv_none_latest_served_duty_implies_none_current_att_duty_body(process)
+    ensures inv_none_latest_served_duty_implies_none_current_att_duty_body(process')
     { }  
 
-    lemma lemma_inv8_f_check_for_next_queued_duty(
+    lemma lemma_inv_none_latest_served_duty_implies_none_current_att_duty_f_check_for_next_queued_duty(
         process: DVCState,
         process': DVCState
     )
     requires f_check_for_next_queued_duty.requires(process)
     requires process' == f_check_for_next_queued_duty(process).state    
-    requires inv8_body(process)
-    ensures inv8_body(process')
+    requires inv_none_latest_served_duty_implies_none_current_att_duty_body(process)
+    ensures inv_none_latest_served_duty_implies_none_current_att_duty_body(process')
     decreases process.attestation_duties_queue
     {
         if  && process.attestation_duties_queue != [] 
@@ -819,16 +819,16 @@ module Fnc_Invs_1_26
                             new_attestation_slashing_db
                         )                        
                     );
-                    lemma_inv8_f_check_for_next_queued_duty(process_mod, process');
+                    lemma_inv_none_latest_served_duty_implies_none_current_att_duty_f_check_for_next_queued_duty(process_mod, process');
                 }
                 else
                 { 
                     var process_mod := process.(
                         attestation_duties_queue := process.attestation_duties_queue[1..]
                     );     
-                    assert inv8_body(process_mod);
+                    assert inv_none_latest_served_duty_implies_none_current_att_duty_body(process_mod);
 
-                    lemma_inv8_f_start_next_duty(process_mod, process.attestation_duties_queue[0], process');
+                    lemma_inv_none_latest_served_duty_implies_none_current_att_duty_f_start_next_duty(process_mod, process.attestation_duties_queue[0], process');
                 }
         }
         else
@@ -837,15 +837,15 @@ module Fnc_Invs_1_26
         }
     }
 
-    lemma lemma_inv8_f_serve_attestation_duty(
+    lemma lemma_inv_none_latest_served_duty_implies_none_current_att_duty_f_serve_attestation_duty(
         process: DVCState,
         attestation_duty: AttestationDuty,
         process': DVCState
     )  
     requires f_serve_attestation_duty.requires(process, attestation_duty)
     requires process' == f_serve_attestation_duty(process, attestation_duty).state
-    requires inv8_body(process)
-    ensures inv8_body(process')
+    requires inv_none_latest_served_duty_implies_none_current_att_duty_body(process)
+    ensures inv_none_latest_served_duty_implies_none_current_att_duty_body(process')
     {
         var process_mod := process.(
                 attestation_duties_queue := process.attestation_duties_queue + [attestation_duty],
@@ -853,10 +853,10 @@ module Fnc_Invs_1_26
             );        
         
 
-        lemma_inv8_f_check_for_next_queued_duty(process_mod, process');        
+        lemma_inv_none_latest_served_duty_implies_none_current_att_duty_f_check_for_next_queued_duty(process_mod, process');        
     } 
 
-    lemma lemma_inv8_f_att_consensus_decided(
+    lemma lemma_inv_none_latest_served_duty_implies_none_current_att_duty_f_att_consensus_decided(
         process: DVCState,
         id: Slot,
         decided_attestation_data: AttestationData, 
@@ -864,8 +864,8 @@ module Fnc_Invs_1_26
     )
     requires f_att_consensus_decided.requires(process, id, decided_attestation_data)
     requires process' == f_att_consensus_decided(process, id, decided_attestation_data).state     
-    requires inv8_body(process)
-    ensures inv8_body(process')
+    requires inv_none_latest_served_duty_implies_none_current_att_duty_body(process)
+    ensures inv_none_latest_served_duty_implies_none_current_att_duty_body(process')
     {
         
         if  && process.current_attestation_duty.isPresent()
@@ -894,36 +894,36 @@ module Fnc_Invs_1_26
                     )
                 );
 
-            assert inv8_body(process);
+            assert inv_none_latest_served_duty_implies_none_current_att_duty_body(process);
 
             var ret_check_for_next_queued_duty := f_check_for_next_queued_duty(process);
             
-            lemma_inv8_f_check_for_next_queued_duty(process, ret_check_for_next_queued_duty.state);
+            lemma_inv_none_latest_served_duty_implies_none_current_att_duty_f_check_for_next_queued_duty(process, ret_check_for_next_queued_duty.state);
 
             assert process' == ret_check_for_next_queued_duty.state;
         }
     }  
 
-    lemma lemma_inv8_f_listen_for_attestation_shares(
+    lemma lemma_inv_none_latest_served_duty_implies_none_current_att_duty_f_listen_for_attestation_shares(
         process: DVCState,
         attestation_share: AttestationShare,
         process': DVCState
     )
     requires f_listen_for_attestation_shares.requires(process, attestation_share)
     requires process' == f_listen_for_attestation_shares(process, attestation_share).state
-    requires inv8_body(process)
-    ensures inv8_body(process')
+    requires inv_none_latest_served_duty_implies_none_current_att_duty_body(process)
+    ensures inv_none_latest_served_duty_implies_none_current_att_duty_body(process')
     {}
 
-    lemma lemma_inv8_f_listen_for_new_imported_blocks(
+    lemma lemma_inv_none_latest_served_duty_implies_none_current_att_duty_f_listen_for_new_imported_blocks(
         process: DVCState,
         block: BeaconBlock,
         process': DVCState
     )
     requires f_listen_for_new_imported_blocks.requires(process, block)
     requires process' == f_listen_for_new_imported_blocks(process, block).state    
-    requires inv8_body(process)
-    ensures inv8_body(process')
+    requires inv_none_latest_served_duty_implies_none_current_att_duty_body(process)
+    ensures inv_none_latest_served_duty_implies_none_current_att_duty_body(process')
     {
         var new_consensus_instances_already_decided := f_listen_for_new_imported_blocks_helper_1(process, block);
 
@@ -943,7 +943,7 @@ module Fnc_Invs_1_26
                     rcvd_attestation_shares := process.rcvd_attestation_shares - att_consensus_instances_already_decided.Keys                    
                 );    
 
-        assert inv8_body(process);
+        assert inv_none_latest_served_duty_implies_none_current_att_duty_body(process);
                     
 
         if process.current_attestation_duty.isPresent() && process.current_attestation_duty.safe_get().slot in att_consensus_instances_already_decided
@@ -959,34 +959,34 @@ module Fnc_Invs_1_26
                 )                
             );
             
-            assert inv8_body(process);
+            assert inv_none_latest_served_duty_implies_none_current_att_duty_body(process);
 
-            lemma_inv8_f_check_for_next_queued_duty(process, process');
+            lemma_inv_none_latest_served_duty_implies_none_current_att_duty_f_check_for_next_queued_duty(process, process');
         }
         else
         {   
-            assert inv8_body(process);
+            assert inv_none_latest_served_duty_implies_none_current_att_duty_body(process);
         }
     }  
 
-    lemma lemma_inv8_f_resend_attestation_share(
+    lemma lemma_inv_none_latest_served_duty_implies_none_current_att_duty_f_resend_attestation_share(
         process: DVCState,
         process': DVCState)
     requires f_resend_attestation_share.requires(process)
     requires process' == f_resend_attestation_share(process).state    
-    requires inv8_body(process)
-    ensures inv8_body(process')
+    requires inv_none_latest_served_duty_implies_none_current_att_duty_body(process)
+    ensures inv_none_latest_served_duty_implies_none_current_att_duty_body(process')
     { }       
          
-    lemma lemma_inv8_add_block_to_bn(
+    lemma lemma_inv_none_latest_served_duty_implies_none_current_att_duty_add_block_to_bn(
         s: DVCState,
         block: BeaconBlock,
         s': DVCState 
     )
     requires add_block_to_bn.requires(s, block)
     requires s' == add_block_to_bn(s, block)
-    requires inv8_body(s)
-    ensures inv8_body(s')
+    requires inv_none_latest_served_duty_implies_none_current_att_duty_body(s)
+    ensures inv_none_latest_served_duty_implies_none_current_att_duty_body(s')
     { }    
 
     lemma lemma_inv_current_att_duty_is_either_none_or_latest_served_duty_f_start_next_duty(process: DVCState, attestation_duty: AttestationDuty, process': DVCState)
@@ -1050,7 +1050,7 @@ module Fnc_Invs_1_26
     )  
     requires f_serve_attestation_duty.requires(process, attestation_duty)
     requires process' == f_serve_attestation_duty(process, attestation_duty).state
-    requires inv8_body(process)  
+    requires inv_none_latest_served_duty_implies_none_current_att_duty_body(process)  
     requires inv_current_att_duty_is_either_none_or_latest_served_duty_body(process)
     ensures inv_current_att_duty_is_either_none_or_latest_served_duty_body(process')
     {
@@ -1256,7 +1256,7 @@ module Fnc_Invs_1_26
     )  
     requires f_serve_attestation_duty.requires(process, attestation_duty)
     requires process' == f_serve_attestation_duty(process, attestation_duty).state
-    requires inv8_body(process)  
+    requires inv_none_latest_served_duty_implies_none_current_att_duty_body(process)  
     requires inv_not_none_current_att_duty_is_latest_served_att_duty_body(process)
     ensures inv_not_none_current_att_duty_is_latest_served_att_duty_body(process')
     {
@@ -1408,7 +1408,7 @@ module Fnc_Invs_1_26
     lemma lemma_inv_no_queued_att_duty_if_latest_served_att_duty_is_none_f_start_next_duty(process: DVCState, attestation_duty: AttestationDuty, process': DVCState)
     requires f_start_next_duty.requires(process, attestation_duty)
     requires process' == f_start_next_duty(process, attestation_duty).state        
-    requires inv8_body(process) || inv_no_queued_att_duty_if_latest_served_att_duty_is_none_body(process)
+    requires inv_none_latest_served_duty_implies_none_current_att_duty_body(process) || inv_no_queued_att_duty_if_latest_served_att_duty_is_none_body(process)
     ensures inv_no_queued_att_duty_if_latest_served_att_duty_is_none_body(process')
     { }  
 
@@ -1418,7 +1418,7 @@ module Fnc_Invs_1_26
     )
     requires f_check_for_next_queued_duty.requires(process)
     requires process' == f_check_for_next_queued_duty(process).state    
-    requires inv8_body(process) || inv_no_queued_att_duty_if_latest_served_att_duty_is_none_body(process)
+    requires inv_none_latest_served_duty_implies_none_current_att_duty_body(process) || inv_no_queued_att_duty_if_latest_served_att_duty_is_none_body(process)
     ensures inv_no_queued_att_duty_if_latest_served_att_duty_is_none_body(process')
     decreases process.attestation_duties_queue
     {
@@ -1448,7 +1448,7 @@ module Fnc_Invs_1_26
                     var process_mod := process.(
                         attestation_duties_queue := process.attestation_duties_queue[1..]
                     );     
-                    assert inv8_body(process_mod) || inv_no_queued_att_duty_if_latest_served_att_duty_is_none_body(process_mod);
+                    assert inv_none_latest_served_duty_implies_none_current_att_duty_body(process_mod) || inv_no_queued_att_duty_if_latest_served_att_duty_is_none_body(process_mod);
 
                     lemma_inv_no_queued_att_duty_if_latest_served_att_duty_is_none_f_start_next_duty(process_mod, process.attestation_duties_queue[0], process');
                 }
@@ -1466,7 +1466,7 @@ module Fnc_Invs_1_26
     )  
     requires f_serve_attestation_duty.requires(process, attestation_duty)
     requires process' == f_serve_attestation_duty(process, attestation_duty).state
-    requires inv8_body(process)  
+    requires inv_none_latest_served_duty_implies_none_current_att_duty_body(process)  
     requires inv_no_queued_att_duty_if_latest_served_att_duty_is_none_body(process)
     ensures inv_no_queued_att_duty_if_latest_served_att_duty_is_none_body(process')
     {
@@ -1658,7 +1658,7 @@ module Fnc_Invs_1_26
                     var process_mod := process.(
                         attestation_duties_queue := process.attestation_duties_queue[1..]
                     );     
-                    assert inv8_body(process_mod) || inv_strictly_increasing_queue_of_att_duties_body(process_mod);
+                    assert inv_none_latest_served_duty_implies_none_current_att_duty_body(process_mod) || inv_strictly_increasing_queue_of_att_duties_body(process_mod);
 
                     lemma_inv_strictly_increasing_queue_of_att_duties_f_start_next_duty(process_mod, process.attestation_duties_queue[0], process');
                 }
